theories/Determinism/SmallStepPairParScheduleDeterminism.v
@@ -1,0 +1,1594 @@
+From Stdlib Require Import List.
+From Stdlib Require Import Program.Equality.
+From Stdlib Require Import Sets.Ensembles.
+From stdpp Require Import gmap.
+
+Require Import theories.Core.DynamicActions.
+Require Import theories.Core.ComputedActions.
+Require Import theories.Core.Expressions.
+Require Import theories.Core.Values.
+Require Import theories.Runtime.Heap.
+Require Import theories.Runtime.TraceSemantics.
+Require Import theories.Runtime.SmallStep.
+Require Import theories.Runtime.SmallStepFacts.
+Require Import theories.Runtime.SmallStepParallel.
+Require Import theories.Runtime.SmallStepSequentialSoundness.
+Require Import theories.Runtime.SmallStepStructuredTrace.
+Require Import theories.Runtime.SmallStepCorrectness.
+Require Import theories.Meta.HeapFacts.
+Require Import theories.Determinism.Determinism.
+Require Import theories.Determinism.SmallStepStructuredReplay.
+
+Lemma Det_Trace_of_phi_as_list_nil :
+  forall phi,
+    phi_as_list phi = nil ->
+    Det_Trace phi.
+Proof.
+  induction phi as [| da | phi1 IHphi1 phi2 IHphi2
+                   | phi1 IHphi1 phi2 IHphi2]; intros HNil; simpl in HNil.
+  - constructor.
+  - discriminate.
+  - apply app_eq_nil in HNil as [HNil1 HNil2].
+    constructor; [now apply IHphi1 | now apply IHphi2 |].
+    split.
+    + intro HConflict.
+      inversion HConflict as [p1 p2 tr1 tr2 HIn1 _ _]; subst.
+      rewrite HNil1 in HIn1.
+      inversion HIn1.
+    + constructor. intros p1 p2 HIn1 _.
+      rewrite HNil1 in HIn1. inversion HIn1.
+  - apply app_eq_nil in HNil as [HNil1 HNil2].
+    constructor; [now apply IHphi1 | now apply IHphi2].
+Qed.
+
+Lemma Phi_Heap_Steps_empty_as_list_reaches_same_heap :
+  forall phi heap,
+    phi_as_list phi = nil ->
+    (phi, heap) ==>* (Phi_Nil, heap).
+Proof.
+  induction phi as [| da | phi1 IHphi1 phi2 IHphi2
+                   | phi1 IHphi1 phi2 IHphi2]; intros heap HNil; simpl in HNil.
+  - exists 0. constructor.
+  - discriminate.
+  - apply app_eq_nil in HNil as [HNil1 HNil2].
+    eapply structured_phi_par_steps.
+    + now apply IHphi1.
+    + now apply IHphi2.
+  - apply app_eq_nil in HNil as [HNil1 HNil2].
+    eapply structured_phi_seq_steps.
+    + now apply IHphi1.
+    + now apply IHphi2.
+Qed.
+
+Lemma Phi_Heap_Steps_empty_as_list_preserves_heap :
+  forall phi heap heap',
+    phi_as_list phi = nil ->
+    (phi, heap) ==>* (Phi_Nil, heap') ->
+    heap ≡@{Heap} heap'.
+Proof.
+  intros phi heap heap' HNil HSteps.
+  eapply Diamond_Term_Walk.
+  - eapply Phi_Heap_Steps_empty_as_list_reaches_same_heap; eauto.
+  - exact HSteps.
+  - now apply Det_Trace_of_phi_as_list_nil.
+Qed.
+
+Lemma Det_Trace_label_phi :
+  forall label,
+    Det_Trace (label_phi label).
+Proof.
+  intros [| da]; constructor.
+Qed.
+
+Lemma PairParStepsPhi_branch_det_traces :
+  forall state phi_state phi_left phi_right state',
+    PairParStepsPhi state phi_state phi_left phi_right state' ->
+    Det_Trace phi_left /\ Det_Trace phi_right.
+Proof.
+  intros state phi_state phi_left phi_right state' HSteps.
+  induction HSteps as
+    [state
+    | state label state' phi_state phi_left phi_right state'' HStep _ IH
+    | left right k label left' phi_state phi_left phi_right state''
+        HStep _ IH
+    | left right k label right' phi_state phi_left phi_right state''
+        HStep _ IH
+    | heap v1 v2 k phi_state phi_left phi_right state'' _ IH].
+  - split; constructor.
+  - exact IH.
+  - destruct IH as [HDetLeft HDetRight].
+    split; [constructor; [apply Det_Trace_label_phi | exact HDetLeft] |
+            exact HDetRight].
+  - destruct IH as [HDetLeft HDetRight].
+    split; [exact HDetLeft |
+            constructor; [apply Det_Trace_label_phi | exact HDetRight]].
+  - exact IH.
+Qed.
+
+Lemma PairParStepsPhi_state_as_stepsphi :
+  forall state phi_state phi_left phi_right state',
+    PairParStepsPhi
+      (PPS_State state) phi_state phi_left phi_right state' ->
+    phi_left = Phi_Nil /\
+    phi_right = Phi_Nil /\
+    exists state_final,
+      state' = PPS_State state_final /\
+      StepsPhi state phi_state state_final.
+Proof.
+  intros state phi_state phi_left phi_right state' HSteps.
+  dependent induction HSteps.
+  - split; [reflexivity |].
+    split; [reflexivity |].
+    exists state. split; [reflexivity | constructor].
+  - destruct (IHHSteps state' eq_refl)
+      as (HLeftNil & HRightNil & state_final & HFinal & HStepsPhi).
+    split; [exact HLeftNil |].
+    split; [exact HRightNil |].
+    exists state_final. split; [exact HFinal |].
+    econstructor; eauto.
+Qed.
+
+Lemma PairParSteps_state_as_steps :
+  forall state trace state',
+    PairParSteps (PPS_State state) trace state' ->
+    exists state_final,
+      state' = PPS_State state_final /\
+      Steps state trace state_final.
+Proof.
+  intros state trace state' HSteps.
+  remember (PPS_State state) as pstate eqn:HPState.
+  revert state HPState.
+  induction HSteps as
+    [pstate
+    | pstate label pstate1 trace pstate2 HStep HSteps IH];
+    intros state0 HPState; subst.
+  - exists state0. split; [reflexivity | constructor].
+  - inversion HStep; subst.
+    destruct (IH state' eq_refl)
+      as (state_final & HFinal & HStepsState).
+    exists state_final. split; [exact HFinal |].
+    econstructor; eauto.
+Qed.
+
+Lemma PairParSteps_run_kdone_terminal_pair_value :
+  forall left right trace heap v,
+    PairParSteps
+      (PPS_Run left right KDone)
+      trace
+      (PPS_State (StDone heap v)) ->
+    exists v1 v2,
+      v = Pair (v1, v2).
+Proof.
+  intros left right trace heap v HSteps.
+  dependent induction HSteps generalizing left right.
+  inversion H; subst; try solve [eapply IHHSteps; reflexivity].
+  destruct
+    (PairParSteps_state_as_steps
+      (StReturn heap0 (Pair (v1, v2)) KDone)
+      trace
+      (PPS_State (StDone heap v)) HSteps)
+    as (state_final & HFinal & HStepsState).
+  inversion HFinal; subst.
+  destruct
+    (Steps_terminal_deterministic
+      (StReturn heap0 (Pair (v1, v2)) KDone)
+      trace heap v
+      nil heap0 (Pair (v1, v2)))
+    as (_ & _ & Hv).
+  - exact HStepsState.
+  - replace nil with (label_trace Silent ++ nil) by reflexivity.
+    econstructor.
+    + constructor.
+    + constructor.
+  - exists v1, v2. exact Hv.
+Qed.
+
+Lemma PairParStepsPhi_run_kdone_terminal_pair_value :
+  forall left right phi_state phi_left phi_right heap v,
+    PairParStepsPhi
+      (PPS_Run left right KDone)
+      phi_state phi_left phi_right
+      (PPS_State (StDone heap v)) ->
+    exists v1 v2,
+      v = Pair (v1, v2).
+Proof.
+  intros left right phi_state phi_left phi_right heap v HSteps.
+  destruct (PairParStepsPhi_as_pairpar_steps_exists _ _ _ _ _ HSteps)
+    as (trace & HPairSteps).
+  eapply PairParSteps_run_kdone_terminal_pair_value; eauto.
+Qed.
+
+Definition label_result_heap (label : Label) (heap : Heap) : Heap :=
+  match label with
+  | Silent => heap
+  | Act (DA_Alloc r l v) => update_H ((r, l), v) heap
+  | Act (DA_Read _ _ _) => heap
+  | Act (DA_Write r l v) => update_H ((r, l), v) heap
+  end.
+
+Definition LabelHeapSafe (label : Label) (heap : Heap) : Prop :=
+  match label with
+  | Silent => True
+  | Act (DA_Alloc r l _) => allocate_H heap r = l
+  | Act (DA_Read r l v) => find_H (r, l) heap = Some v
+  | Act (DA_Write r l _) => find_H (r, l) heap <> None
+  end.
+
+Lemma Step_label_heap_safe :
+  forall state label state',
+    Step state label state' ->
+    LabelHeapSafe label (state_heap state).
+Proof.
+  intros state label state' HStep.
+  inversion HStep; subst; simpl; auto.
+Qed.
+
+Lemma Step_rebase_with_safe_label :
+  forall state label state' heap,
+    Step state label state' ->
+    LabelHeapSafe label heap ->
+    Step
+      (with_state_heap heap state)
+      label
+      (with_state_heap (label_result_heap label heap) state').
+Proof.
+  intros state label state' heap HStep HSafe.
+  inversion HStep; subst; simpl in *; try (constructor; eauto; fail).
+Qed.
+
+Lemma Step_unbase_with_safe_label :
+  forall state heap label state',
+    Step (with_state_heap heap state) label state' ->
+    LabelHeapSafe label (state_heap state) ->
+    Step state label
+      (with_state_heap (label_result_heap label (state_heap state)) state').
+Proof.
+  intros state heap label state' HStep HSafe.
+  destruct state as [heap0 env rho e k | heap0 v k | heap0 v];
+    simpl in *;
+    inversion HStep; subst; simpl in *; try (constructor; eauto; fail).
+Qed.
+
+Lemma Step_silent_preserves_heap :
+  forall state state',
+    Step state Silent state' ->
+    state_heap state' = state_heap state.
+Proof.
+  intros state state' HStep.
+  inversion HStep; subst; reflexivity.
+Qed.
+
+Lemma Disjoint_Traces_single_inv :
+  forall da1 da2,
+    Disjoint_Traces (da1 :: nil) (da2 :: nil) ->
+    Disjoint_Dynamic da1 da2.
+Proof.
+  intros da1 da2 HDisjoint.
+  inversion HDisjoint as [tr1 tr2 HAll]; subst.
+  apply HAll; simpl; auto.
+Qed.
+
+Lemma Disjoint_Dynamic_sym :
+  forall da1 da2,
+    Disjoint_Dynamic da1 da2 ->
+    Disjoint_Dynamic da2 da1.
+Proof.
+  destruct da1 as [r1 l1 v1 | r1 l1 v1 | r1 l1 v1];
+    destruct da2 as [r2 l2 v2 | r2 l2 v2 | r2 l2 v2];
+    intro HDisjoint; inversion HDisjoint; subst; constructor;
+    try assumption;
+    match goal with
+    | HNeq : ?x <> ?y |- ?y <> ?x =>
+        intro HSame; apply HNeq; symmetry; exact HSame
+    end.
+Qed.
+
+Lemma Disjoint_Traces_sym :
+  forall trace1 trace2,
+    Disjoint_Traces trace1 trace2 ->
+    Disjoint_Traces trace2 trace1.
+Proof.
+  intros trace1 trace2 HDisjoint.
+  inversion HDisjoint as [tr1 tr2 HAll]; subst.
+  constructor.
+  intros p2 p1 HIn2 HIn1.
+  apply Disjoint_Dynamic_sym.
+  eapply HAll; eauto.
+Qed.
+
+Lemma PairParCheckPass_sound_disjoint_traces :
+  forall phi_left phi_right theta_left theta_right,
+    phi_left ⋞ theta_left ->
+    phi_right ⋞ theta_right ->
+    PairParCheckPass theta_left theta_right ->
+    Disjoint_Traces (phi_as_list phi_left) (phi_as_list phi_right).
+Proof.
+  intros phi_left phi_right theta_left theta_right
+    HSoundLeft HSoundRight [HDisjoint _].
+  eapply Phi_Theta_Disjointness_disjoint_traces; eauto.
+Qed.
+
+Lemma PairParCheckPass_sound_disjoint_traces_sym :
+  forall phi_left phi_right theta_left theta_right,
+    phi_left ⋞ theta_left ->
+    phi_right ⋞ theta_right ->
+    PairParCheckPass theta_left theta_right ->
+    Disjoint_Traces (phi_as_list phi_right) (phi_as_list phi_left).
+Proof.
+  intros phi_left phi_right theta_left theta_right
+    HSoundLeft HSoundRight HPass.
+  apply Disjoint_Traces_sym.
+  eapply PairParCheckPass_sound_disjoint_traces; eauto.
+Qed.
+
+Lemma LabelHeapSafe_alloc_preserved_by_alloc :
+  forall heap r1 l1 v1 r2 l2 v2,
+    allocate_H heap r1 = l1 ->
+    allocate_H heap r2 = l2 ->
+    Disjoint_Dynamic (DA_Alloc r1 l1 v1) (DA_Alloc r2 l2 v2) ->
+    allocate_H (update_H ((r2, l2), v2) heap) r1 = l1.
+Proof.
+  intros heap r1 l1 v1 r2 l2 v2 HSafe HOther HDynamic.
+  destruct (Nat.eq_dec r1 r2) as [HRegion | HRegion].
+  - subst r1.
+    assert (l1 = l2) by congruence.
+    subst l1.
+    inversion HDynamic; subst.
+    match goal with
+    | HNeq : (_, _) <> (_, _) |- _ =>
+        exfalso; apply HNeq; reflexivity
+    end.
+  - rewrite allocate_H_update_fresh_different_region;
+      [exact HSafe | intro H; apply HRegion; symmetry; exact H |].
+    rewrite <- HOther.
+    apply allocate_H_fresh.
+Qed.
+
+Lemma allocate_H_update_existing_nonnone :
+  forall heap r k value,
+    find_H k heap <> None ->
+    allocate_H (update_H (k, value) heap) r = allocate_H heap r.
+Proof.
+  intros heap r k value HExists.
+  destruct (find_H k heap) as [old |] eqn:HFind.
+  - apply allocate_H_update_existing with (old_value := old).
+    exact HFind.
+  - contradiction.
+Qed.
+
+Lemma find_H_some_update_ne :
+  forall heap k k_update v_update v,
+    k <> k_update ->
+    find_H k heap = Some v ->
+    find_H k (update_H (k_update, v_update) heap) = Some v.
+Proof.
+  intros heap k k_update v_update v HNe HFind.
+  apply H_diff_keys_2; [| exact HFind].
+  intro HEq.
+  apply HNe.
+  symmetry.
+  exact HEq.
+Qed.
+
+Lemma find_H_some_update_ne_reflect :
+  forall heap k k_update v_update v,
+    k <> k_update ->
+    find_H k (update_H (k_update, v_update) heap) = Some v ->
+    find_H k heap = Some v.
+Proof.
+  intros heap k k_update v_update v HNe HFind.
+  eapply H_diff_keys_1; eauto.
+Qed.
+
+Lemma find_H_exists_update_preserved :
+  forall heap k k_update v_update,
+    find_H k heap <> None ->
+    find_H k (update_H (k_update, v_update) heap) <> None.
+Proof.
+  intros heap k k_update v_update HExists HNone.
+  unfold find_H, update_H in *.
+  apply lookup_insert_None in HNone.
+  destruct HNone as [HOldNone _].
+  apply HExists.
+  exact HOldNone.
+Qed.
+
+Lemma find_H_exists_update_reflected_ne :
+  forall heap k k_update v_update,
+    k <> k_update ->
+    find_H k (update_H (k_update, v_update) heap) <> None ->
+    find_H k heap <> None.
+Proof.
+  intros heap k k_update v_update HNe HExists HNone.
+  apply HExists.
+  unfold find_H, update_H in *.
+  apply lookup_insert_None.
+  split.
+  - exact HNone.
+  - intro HEq. apply HNe. symmetry. exact HEq.
+Qed.
+
+Lemma read_safe_preserved_by_disjoint_alloc :
+  forall heap r1 l1 v1 r2 l2 v2,
+    find_H (r1, l1) heap = Some v1 ->
+    Disjoint_Dynamic (DA_Read r1 l1 v1) (DA_Alloc r2 l2 v2) ->
+    find_H (r1, l1) (update_H ((r2, l2), v2) heap) = Some v1.
+Proof.
+  intros heap r1 l1 v1 r2 l2 v2 HFind HDynamic.
+  inversion HDynamic; subst.
+  apply find_H_some_update_ne; assumption.
+Qed.
+
+Lemma read_safe_reflected_by_disjoint_alloc :
+  forall heap r1 l1 v1 r2 l2 v2,
+    find_H (r1, l1) (update_H ((r2, l2), v2) heap) = Some v1 ->
+    Disjoint_Dynamic (DA_Read r1 l1 v1) (DA_Alloc r2 l2 v2) ->
+    find_H (r1, l1) heap = Some v1.
+Proof.
+  intros heap r1 l1 v1 r2 l2 v2 HFind HDynamic.
+  inversion HDynamic; subst.
+  apply find_H_some_update_ne_reflect with (k_update := (r2, l2)) (v_update := v2);
+    assumption.
+Qed.
+
+Lemma read_safe_preserved_by_disjoint_write :
+  forall heap r1 l1 v1 r2 l2 v2,
+    find_H (r1, l1) heap = Some v1 ->
+    Disjoint_Dynamic (DA_Read r1 l1 v1) (DA_Write r2 l2 v2) ->
+    find_H (r1, l1) (update_H ((r2, l2), v2) heap) = Some v1.
+Proof.
+  intros heap r1 l1 v1 r2 l2 v2 HFind HDynamic.
+  inversion HDynamic; subst.
+  apply find_H_some_update_ne; assumption.
+Qed.
+
+Lemma read_safe_reflected_by_disjoint_write :
+  forall heap r1 l1 v1 r2 l2 v2,
+    find_H (r1, l1) (update_H ((r2, l2), v2) heap) = Some v1 ->
+    Disjoint_Dynamic (DA_Read r1 l1 v1) (DA_Write r2 l2 v2) ->
+    find_H (r1, l1) heap = Some v1.
+Proof.
+  intros heap r1 l1 v1 r2 l2 v2 HFind HDynamic.
+  inversion HDynamic; subst.
+  apply find_H_some_update_ne_reflect with (k_update := (r2, l2)) (v_update := v2);
+    assumption.
+Qed.
+
+Definition LabelAllocReflectionStable (label other_label : Label) : Prop :=
+  match label, other_label with
+  | Act (DA_Alloc r1 _ _), Act (DA_Alloc r2 _ _) => r2 <> r1
+  | _, _ => True
+  end.
+
+Lemma DA_alloc_in_theta_alloc_abs :
+  forall r l v acts,
+    DA_in_Theta (DA_Alloc r l v) (Some acts) ->
+    set_elem acts (CA_AllocAbs r).
+Proof.
+  intros r l v acts HIn.
+  dependent induction HIn; try discriminate; try solve [inversion x].
+  - assumption.
+  - unfold set_elem, set_union.
+    apply Union_introl. eapply IHHIn; reflexivity.
+  - unfold set_elem, set_union.
+    apply Union_intror. eapply IHHIn; reflexivity.
+Qed.
+
+Lemma LabelAllocReflectionStable_from_theta :
+  forall label_left label_right theta_left theta_right,
+    label_phi label_left ⋞ theta_left ->
+    label_phi label_right ⋞ theta_right ->
+    Disjointness theta_left theta_right ->
+    LabelAllocReflectionStable label_right label_left.
+Proof.
+  intros label_left label_right theta_left theta_right
+    HSoundLeft HSoundRight HDisjoint.
+  destruct label_right as [| da_right]; [exact I |].
+  destruct label_left as [| da_left]; [destruct da_right; exact I |].
+  destruct da_right as [rR lR vR | rR lR vR | rR lR vR];
+    destruct da_left as [rL lL vL | rL lL vL | rL lL vL];
+    simpl; try exact I.
+  inversion HDisjoint as [acts_left acts_right HDisjointSets]; subst.
+  assert (HLeftIn :
+    DA_in_Theta (DA_Alloc rL lL vL) (Some acts_left)).
+  {
+    eapply Phi_Theta_Soundness_da_in; eauto.
+    constructor.
+  }
+  assert (HRightIn :
+    DA_in_Theta (DA_Alloc rR lR vR) (Some acts_right)).
+  {
+    eapply Phi_Theta_Soundness_da_in; eauto.
+    constructor.
+  }
+  pose proof
+    (DA_alloc_in_theta_alloc_abs rL lL vL acts_left HLeftIn)
+    as HLeftAlloc.
+  pose proof
+    (DA_alloc_in_theta_alloc_abs rR lR vR acts_right HRightIn)
+    as HRightAlloc.
+  inversion HDisjointSets as [acts1 acts2 HAll]; subst.
+  pose proof
+    (HAll (CA_AllocAbs rL) (CA_AllocAbs rR)
+      HLeftAlloc HRightAlloc)
+    as HComputedDisjoint.
+  inversion HComputedDisjoint; subst.
+  exact H1.
+Qed.
+
+Lemma LabelHeapSafe_preserved_by_disjoint_step :
+  forall label other other_label other',
+    Step other other_label other' ->
+    LabelHeapSafe label (state_heap other) ->
+    Disjoint_Traces (label_trace label) (label_trace other_label) ->
+    LabelHeapSafe label (state_heap other').
+Proof.
+  intros label other other_label other' HStep HSafe HDisjoint.
+  destruct label as [| da].
+  - exact I.
+  - destruct other_label as [| da_other].
+    + pose proof (Step_silent_preserves_heap other other' HStep) as HHeap.
+      simpl in *. now rewrite HHeap.
+    + pose proof (Disjoint_Traces_single_inv da da_other HDisjoint)
+        as HDynamic.
+      pose proof HSafe as HSafe0.
+      destruct da_other as [rO lO vO | rO lO vO | rO lO vO].
+      * inversion HStep; subst; simpl in *; try exact HSafe0.
+        destruct da as [rA lA vA | rA lA vA | rA lA vA]; simpl in *.
+        -- eapply LabelHeapSafe_alloc_preserved_by_alloc; eauto.
+        -- eapply read_safe_preserved_by_disjoint_alloc; eauto.
+        -- apply find_H_exists_update_preserved.
+           exact HSafe0.
+      * inversion HStep; subst; simpl in *; exact HSafe0.
+      * inversion HStep; subst; simpl in *; try exact HSafe0.
+        destruct da as [rA lA vA | rA lA vA | rA lA vA]; simpl in *.
+        -- rewrite allocate_H_update_existing_nonnone.
+           ++ exact HSafe0.
+           ++ assumption.
+        -- eapply read_safe_preserved_by_disjoint_write; eauto.
+        -- apply find_H_exists_update_preserved.
+           exact HSafe0.
+Qed.
+
+Lemma Step_state_heap_label_result :
+  forall state label state',
+    Step state label state' ->
+    state_heap state' = label_result_heap label (state_heap state).
+Proof.
+  intros state label state' HStep.
+  inversion HStep; subst; simpl; reflexivity.
+Qed.
+
+Lemma LabelHeapSafe_reflected_by_disjoint_step :
+  forall label other other_label other',
+    Step other other_label other' ->
+    LabelAllocReflectionStable label other_label ->
+    LabelHeapSafe label (state_heap other') ->
+    Disjoint_Traces (label_trace label) (label_trace other_label) ->
+    LabelHeapSafe label (state_heap other).
+Proof.
+  intros label other other_label other' HStep HStable HSafe HDisjoint.
+  destruct label as [| da].
+  - exact I.
+  - destruct other_label as [| da_other].
+    + pose proof (Step_silent_preserves_heap other other' HStep) as HHeap.
+      simpl in *. now rewrite <- HHeap.
+    + pose proof (Disjoint_Traces_single_inv da da_other HDisjoint)
+        as HDynamic.
+      pose proof HSafe as HSafe0.
+      pose proof (Step_state_heap_label_result _ _ _ HStep) as HHeapResult.
+      pose proof (Step_label_heap_safe _ _ _ HStep) as HOtherSafe.
+      destruct da_other as [rO lO vO | rO lO vO | rO lO vO].
+      * simpl in HHeapResult, HOtherSafe.
+        rewrite HHeapResult in HSafe0.
+        simpl in HSafe0.
+        destruct da as [rA lA vA | rA lA vA | rA lA vA]; simpl in *.
+        -- rewrite <- (allocate_H_update_fresh_different_region
+             (state_heap other) rA rO lO vO).
+           ++ exact HSafe0.
+           ++ exact HStable.
+           ++ rewrite <- HOtherSafe. apply allocate_H_fresh.
+        -- eapply read_safe_reflected_by_disjoint_alloc; eauto.
+        -- inversion HDynamic; subst.
+           eapply find_H_exists_update_reflected_ne; eauto.
+      * simpl in HHeapResult.
+        rewrite HHeapResult in HSafe0.
+        exact HSafe0.
+      * simpl in HHeapResult, HOtherSafe.
+        rewrite HHeapResult in HSafe0.
+        simpl in HSafe0.
+        destruct da as [rA lA vA | rA lA vA | rA lA vA]; simpl in *.
+        -- rewrite allocate_H_update_existing_nonnone in HSafe0.
+           ++ exact HSafe0.
+           ++ exact HOtherSafe.
+        -- eapply read_safe_reflected_by_disjoint_write; eauto.
+        -- inversion HDynamic; subst.
+           eapply find_H_exists_update_reflected_ne; eauto.
+Qed.
+
+Ltac solve_label_update_commute :=
+  unfold update_H; simpl;
+  apply insert_commute;
+  match goal with
+  | HNeq : ?k1 <> ?k2 |- ?k1 <> ?k2 =>
+      exact HNeq
+  | HNeq : ?k1 <> ?k2 |- ?k2 <> ?k1 =>
+      let HSame := fresh "HSame" in
+      intro HSame; apply HNeq; symmetry; exact HSame
+  end.
+
+Lemma label_result_heap_commute_disjoint :
+  forall label1 label2 heap,
+    Disjoint_Traces (label_trace label1) (label_trace label2) ->
+    label_result_heap label2 (label_result_heap label1 heap) ≡@{Heap}
+    label_result_heap label1 (label_result_heap label2 heap).
+Proof.
+  intros label1 label2 heap HDisjoint.
+  destruct label1 as [| da1]; destruct label2 as [| da2];
+    simpl in *; try reflexivity.
+  pose proof (Disjoint_Traces_single_inv da1 da2 HDisjoint) as HDynamic.
+  destruct da1 as [r1 l1 v1 | r1 l1 v1 | r1 l1 v1];
+    destruct da2 as [r2 l2 v2 | r2 l2 v2 | r2 l2 v2];
+    simpl in *; try reflexivity;
+    inversion HDynamic; subst; solve_label_update_commute.
+Qed.
+
+Ltac solve_label_update_commute_eq :=
+  unfold update_H; simpl;
+  apply insert_commute;
+  match goal with
+  | HNeq : ?k1 <> ?k2 |- ?k1 <> ?k2 =>
+      exact HNeq
+  | HNeq : ?k1 <> ?k2 |- ?k2 <> ?k1 =>
+      let HSame := fresh "HSame" in
+      intro HSame; apply HNeq; symmetry; exact HSame
+  end.
+
+Lemma label_result_heap_commute_disjoint_eq :
+  forall label1 label2 heap,
+    Disjoint_Traces (label_trace label1) (label_trace label2) ->
+    label_result_heap label2 (label_result_heap label1 heap) =
+    label_result_heap label1 (label_result_heap label2 heap).
+Proof.
+  intros label1 label2 heap HDisjoint.
+  destruct label1 as [| da1]; destruct label2 as [| da2];
+    simpl in *; try reflexivity.
+  pose proof (Disjoint_Traces_single_inv da1 da2 HDisjoint) as HDynamic.
+  destruct da1 as [r1 l1 v1 | r1 l1 v1 | r1 l1 v1];
+    destruct da2 as [r2 l2 v2 | r2 l2 v2 | r2 l2 v2];
+    simpl in *; try reflexivity;
+    inversion HDynamic; subst; solve_label_update_commute_eq.
+Qed.
+
+Lemma Step_rebase_after_disjoint_step :
+  forall state label state' other other_label other',
+    state_heap state = state_heap other ->
+    Step state label state' ->
+    Step other other_label other' ->
+    Disjoint_Traces (label_trace label) (label_trace other_label) ->
+    Step
+      (with_state_heap (state_heap other') state)
+      label
+      (with_state_heap (label_result_heap label (state_heap other')) state').
+Proof.
+  intros state label state' other other_label other'
+    HHeapAgree HStepState HStepOther HDisjoint.
+  eapply Step_rebase_with_safe_label.
+  - exact HStepState.
+  - eapply LabelHeapSafe_preserved_by_disjoint_step; eauto.
+    rewrite <- HHeapAgree.
+    eapply Step_label_heap_safe; eauto.
+Qed.
+
+Lemma PairParLeftRightStep_local_diamond :
+  forall left right k label_left label_right left' right',
+    state_heap left = state_heap right ->
+    Step left label_left left' ->
+    Step right label_right right' ->
+    Disjoint_Traces (label_trace label_left) (label_trace label_right) ->
+    Disjoint_Traces (label_trace label_right) (label_trace label_left) ->
+    exists state_after,
+      PairParStep
+        (PPS_Run left' (with_state_heap (state_heap left') right) k)
+        label_right
+        state_after /\
+      PairParStep
+        (PPS_Run (with_state_heap (state_heap right') left) right' k)
+        label_left
+        state_after.
+Proof.
+  intros left right k label_left label_right left' right'
+    HHeapAgree HStepLeft HStepRight HDisjointLR HDisjointRL.
+  set (heap_after :=
+    label_result_heap label_right
+      (label_result_heap label_left (state_heap left))).
+  set (state_after :=
+    PPS_Run
+      (with_state_heap heap_after left')
+      (with_state_heap heap_after right')
+      k).
+  exists state_after.
+  split.
+  - subst state_after.
+    replace (with_state_heap heap_after left') with
+      (with_state_heap
+        (state_heap (with_state_heap heap_after right')) left')
+      by (rewrite state_heap_with_state_heap; reflexivity).
+    apply PPStep_Right.
+    subst heap_after.
+    rewrite <- (Step_state_heap_label_result _ _ _ HStepLeft).
+    eapply (Step_rebase_after_disjoint_step
+      right label_right right' left label_left left').
+    + symmetry. exact HHeapAgree.
+    + exact HStepRight.
+    + exact HStepLeft.
+    + exact HDisjointRL.
+  - subst state_after.
+    replace (with_state_heap heap_after right') with
+      (with_state_heap
+        (state_heap (with_state_heap heap_after left')) right')
+      by (rewrite state_heap_with_state_heap; reflexivity).
+    apply PPStep_Left.
+    subst heap_after.
+    rewrite (label_result_heap_commute_disjoint_eq
+      label_left label_right (state_heap left) HDisjointLR).
+    rewrite HHeapAgree.
+    rewrite <- (Step_state_heap_label_result _ _ _ HStepRight).
+    eapply (Step_rebase_after_disjoint_step
+      left label_left left' right label_right right').
+    + exact HHeapAgree.
+    + exact HStepLeft.
+    + exact HStepRight.
+    + exact HDisjointLR.
+Qed.
+
+Lemma PairParLeftRightActualStep_local_diamond :
+  forall left right label_left label_right left' right_after,
+    state_heap left = state_heap right ->
+    Step left label_left left' ->
+    Step (with_state_heap (state_heap left') right) label_right right_after ->
+    LabelAllocReflectionStable label_right label_left ->
+    Disjoint_Traces (label_trace label_left) (label_trace label_right) ->
+    Disjoint_Traces (label_trace label_right) (label_trace label_left) ->
+    exists right',
+      Step right label_right right' /\
+      Step
+        (with_state_heap (state_heap right') left)
+        label_left
+        (with_state_heap (state_heap right_after) left') /\
+      right_after = with_state_heap (state_heap right_after) right'.
+Proof.
+  intros left right label_left label_right left' right_after
+    HHeapAgree HStepLeft HStepRightAfter HStable HDisjointLR HDisjointRL.
+  pose proof
+    (Step_label_heap_safe _ _ _ HStepRightAfter)
+    as HSafeAfter.
+  rewrite state_heap_with_state_heap in HSafeAfter.
+  pose proof
+    (LabelHeapSafe_reflected_by_disjoint_step
+      label_right left label_left left'
+      HStepLeft HStable HSafeAfter HDisjointRL)
+    as HSafeBefore.
+  set (right' :=
+    with_state_heap
+      (label_result_heap label_right (state_heap right))
+      right_after).
+  assert (HStepRight : Step right label_right right').
+  {
+    subst right'.
+    eapply Step_unbase_with_safe_label.
+    - exact HStepRightAfter.
+    - rewrite <- HHeapAgree. exact HSafeBefore.
+  }
+  exists right'.
+  split; [exact HStepRight |].
+  split.
+  - replace (state_heap right_after) with
+      (label_result_heap label_left (state_heap right')).
+    + eapply (Step_rebase_after_disjoint_step
+        left label_left left' right label_right right').
+      * exact HHeapAgree.
+      * exact HStepLeft.
+      * exact HStepRight.
+      * exact HDisjointLR.
+    + rewrite (Step_state_heap_label_result _ _ _ HStepRightAfter).
+	      rewrite (Step_state_heap_label_result _ _ _ HStepLeft).
+	      rewrite (Step_state_heap_label_result _ _ _ HStepRight).
+	      rewrite HHeapAgree.
+	      rewrite state_heap_with_state_heap.
+	      symmetry.
+	      apply label_result_heap_commute_disjoint_eq.
+      exact HDisjointLR.
+  - subst right'.
+    destruct right_after; reflexivity.
+Qed.
+
+Lemma PairParStepsPhi_LeftRight_adjacent_swap :
+  forall left right k label_left label_right left' right_after
+    phi_state phi_left phi_right final_state,
+    state_heap left = state_heap right ->
+    Step left label_left left' ->
+    Step (with_state_heap (state_heap left') right) label_right right_after ->
+    LabelAllocReflectionStable label_right label_left ->
+    Disjoint_Traces (label_trace label_left) (label_trace label_right) ->
+    Disjoint_Traces (label_trace label_right) (label_trace label_left) ->
+    PairParStepsPhi
+      (PPS_Run (with_state_heap (state_heap right_after) left') right_after k)
+      phi_state phi_left phi_right final_state ->
+    PairParStepsPhi
+      (PPS_Run left right k)
+      phi_state
+      (Phi_Seq (label_phi label_left) phi_left)
+      (Phi_Seq (label_phi label_right) phi_right)
+      final_state.
+Proof.
+  intros left right k label_left label_right left' right_after
+    phi_state phi_left phi_right final_state
+    HHeapAgree HStepLeft HStepRightAfter HStable HDisjointLR HDisjointRL
+    HRest.
+  destruct
+    (PairParLeftRightActualStep_local_diamond
+      left right label_left label_right left' right_after
+      HHeapAgree HStepLeft HStepRightAfter HStable HDisjointLR HDisjointRL)
+    as (right' & HStepRight & HStepLeftAfterRight & HRightAfterRebase).
+  eapply PairParStepsPhi_Right.
+  - exact HStepRight.
+  - eapply PairParStepsPhi_Left.
+    + exact HStepLeftAfterRight.
+    + replace
+        (PPS_Run (with_state_heap (state_heap right_after) left')
+           (with_state_heap
+             (state_heap (with_state_heap (state_heap right_after) left'))
+             right') k)
+        with
+        (PPS_Run (with_state_heap (state_heap right_after) left')
+           right_after k).
+	      * exact HRest.
+	      * rewrite state_heap_with_state_heap.
+	        rewrite <- HRightAfterRebase.
+	        reflexivity.
+Qed.
+
+Lemma PairParStepsPhi_LeftRight_adjacent_swap_checked :
+  forall left right k label_left label_right left' right_after
+    phi_state phi_left phi_right final_state theta_left theta_right,
+    state_heap left = state_heap right ->
+    Step left label_left left' ->
+    Step (with_state_heap (state_heap left') right) label_right right_after ->
+    label_phi label_left ⋞ theta_left ->
+    label_phi label_right ⋞ theta_right ->
+    PairParCheckPass theta_left theta_right ->
+    PairParStepsPhi
+      (PPS_Run (with_state_heap (state_heap right_after) left') right_after k)
+      phi_state phi_left phi_right final_state ->
+    PairParStepsPhi
+      (PPS_Run left right k)
+      phi_state
+      (Phi_Seq (label_phi label_left) phi_left)
+      (Phi_Seq (label_phi label_right) phi_right)
+      final_state.
+Proof.
+  intros left right k label_left label_right left' right_after
+    phi_state phi_left phi_right final_state theta_left theta_right
+    HHeapAgree HStepLeft HStepRightAfter
+    HSoundLeft HSoundRight HPass HRest.
+  eapply PairParStepsPhi_LeftRight_adjacent_swap; eauto.
+  - eapply LabelAllocReflectionStable_from_theta; eauto.
+    destruct HPass as [HDisjoint _]. exact HDisjoint.
+  - rewrite <- (phi_as_list_label_phi label_left).
+    rewrite <- (phi_as_list_label_phi label_right).
+    eapply PairParCheckPass_sound_disjoint_traces; eauto.
+  - rewrite <- (phi_as_list_label_phi label_right).
+    rewrite <- (phi_as_list_label_phi label_left).
+    eapply PairParCheckPass_sound_disjoint_traces_sym; eauto.
+Qed.
+
+Inductive PairParLeftOnlyStepsPhi :
+  PairParState -> Phi -> Phi -> PairParState -> Prop :=
+| PPLO_Refl :
+    forall state,
+      PairParLeftOnlyStepsPhi state Phi_Nil Phi_Nil state
+| PPLO_State :
+    forall state phi_state final_state,
+      PairParStepsPhi
+        (PPS_State state) phi_state Phi_Nil Phi_Nil final_state ->
+      PairParLeftOnlyStepsPhi
+        (PPS_State state) phi_state Phi_Nil final_state
+| PPLO_Left :
+    forall left right k label left' phi_state phi_left final_state,
+      Step left label left' ->
+      PairParLeftOnlyStepsPhi
+        (PPS_Run left' (with_state_heap (state_heap left') right) k)
+        phi_state phi_left final_state ->
+      PairParLeftOnlyStepsPhi
+        (PPS_Run left right k)
+        phi_state
+        (Phi_Seq (label_phi label) phi_left)
+        final_state
+| PPLO_Done :
+    forall heap v1 v2 k phi_state phi_left final_state,
+      PairParLeftOnlyStepsPhi
+        (PPS_State (StReturn heap (Pair (v1, v2)) k))
+        phi_state phi_left final_state ->
+      PairParLeftOnlyStepsPhi
+        (PPS_Run (StDone heap v1) (StDone heap v2) k)
+        phi_state phi_left final_state.
+
+Inductive PairParRightThenLeftStepsPhi :
+  PairParState -> Phi -> Phi -> Phi -> PairParState -> Prop :=
+| PPRTL_LeftOnly :
+    forall state phi_state phi_left final_state,
+      PairParLeftOnlyStepsPhi state phi_state phi_left final_state ->
+      PairParRightThenLeftStepsPhi
+        state phi_state phi_left Phi_Nil final_state
+| PPRTL_Right :
+    forall left right k label right'
+      phi_state phi_left phi_right final_state,
+      Step right label right' ->
+      PairParRightThenLeftStepsPhi
+        (PPS_Run (with_state_heap (state_heap right') left) right' k)
+        phi_state phi_left phi_right final_state ->
+      PairParRightThenLeftStepsPhi
+        (PPS_Run left right k)
+        phi_state
+        phi_left
+        (Phi_Seq (label_phi label) phi_right)
+        final_state.
+
+Lemma PairParLeftOnlyStepsPhi_as_pairpar_steps_phi :
+  forall state phi_state phi_left final_state,
+    PairParLeftOnlyStepsPhi state phi_state phi_left final_state ->
+    PairParStepsPhi state phi_state phi_left Phi_Nil final_state.
+Proof.
+  intros state phi_state phi_left final_state HSteps.
+  induction HSteps.
+  - constructor.
+  - exact H.
+  - eapply PairParStepsPhi_Left; eauto.
+  - eapply PairParStepsPhi_Done; eauto.
+Qed.
+
+Lemma PairParRightThenLeftStepsPhi_as_pairpar_steps_phi :
+  forall state phi_state phi_left phi_right final_state,
+    PairParRightThenLeftStepsPhi
+      state phi_state phi_left phi_right final_state ->
+    PairParStepsPhi state phi_state phi_left phi_right final_state.
+Proof.
+  intros state phi_state phi_left phi_right final_state HSteps.
+  induction HSteps.
+  - now apply PairParLeftOnlyStepsPhi_as_pairpar_steps_phi.
+  - eapply PairParStepsPhi_Right; eauto.
+Qed.
+
+Lemma PairParLeftOnlyStepsPhi_state_as_stepsphi :
+  forall state phi_state phi_left final_state,
+    PairParLeftOnlyStepsPhi
+      (PPS_State state) phi_state phi_left final_state ->
+    phi_left = Phi_Nil /\
+    exists state_final,
+      final_state = PPS_State state_final /\
+      StepsPhi state phi_state state_final.
+Proof.
+  intros state phi_state phi_left final_state HSteps.
+  pose proof
+    (PairParLeftOnlyStepsPhi_as_pairpar_steps_phi
+      (PPS_State state) phi_state phi_left final_state HSteps)
+    as HPairSteps.
+  destruct
+    (PairParStepsPhi_state_as_stepsphi
+      state phi_state phi_left Phi_Nil final_state HPairSteps)
+    as (HLeftNil & _ & state_final & HFinal & HStepsPhi).
+  split; [exact HLeftNil |].
+  exists state_final. split; assumption.
+Qed.
+
+Lemma StepsPhi_return_kdone :
+  forall heap v,
+    StepsPhi
+      (StReturn heap v KDone)
+      (Phi_Seq (label_phi Silent) Phi_Nil)
+      (StDone heap v).
+Proof.
+  intros heap v.
+  eapply StepsPhi_Step.
+  - constructor.
+  - constructor.
+Qed.
+
+Lemma with_state_heap_overwrite :
+  forall heap_outer heap_inner state,
+    with_state_heap heap_outer (with_state_heap heap_inner state) =
+    with_state_heap heap_outer state.
+Proof.
+  intros heap_outer heap_inner state.
+  destruct state; reflexivity.
+Qed.
+
+Lemma PairParLeftOnlyStepsPhi_terminal_decompose_kdone :
+  forall left v_right phi_state phi_left heap_final v_final,
+    PairParLeftOnlyStepsPhi
+      (PPS_Run left (StDone (state_heap left) v_right) KDone)
+      phi_state
+      phi_left
+      (PPS_State (StDone heap_final v_final)) ->
+    exists heap_left v_left,
+      StepsPhi left phi_left (StDone heap_left v_left) /\
+      heap_final = heap_left /\
+      v_final = Pair (v_left, v_right).
+Proof.
+  intros left v_right phi_state phi_left heap_final v_final HSteps.
+  dependent induction HSteps generalizing left v_right heap_final v_final.
+  - destruct
+      (IHHSteps left' v_right heap_final v_final)
+      as (heap_left & v_left & HLeftSteps & HHeapFinal & HValFinal).
+    + simpl. reflexivity.
+    + reflexivity.
+    + exists heap_left, v_left.
+      split.
+      * eapply StepsPhi_Step; eauto.
+      * split; assumption.
+  - destruct
+      (PairParLeftOnlyStepsPhi_state_as_stepsphi
+        (StReturn (state_heap left) (Pair (v1, v_right)) KDone)
+        phi_state phi_left
+        (PPS_State (StDone heap_final v_final)) HSteps)
+      as (HLeftNil & state_final & HStateFinal & HStateSteps).
+    inversion HStateFinal; subst.
+    destruct
+      (StepsPhi_terminal_deterministic
+        (StReturn (state_heap left) (Pair (v1, v_right)) KDone)
+        phi_state heap_final v_final
+        (Phi_Seq (label_phi Silent) Phi_Nil)
+        (state_heap left) (Pair (v1, v_right))
+        HStateSteps
+        (StepsPhi_return_kdone
+          (state_heap left) (Pair (v1, v_right))))
+      as (_ & HHeapEq & HValEq).
+    exists (state_heap left), v1.
+    split.
+    + rewrite <- x.
+      constructor.
+    + split; assumption.
+Qed.
+
+Lemma PairParLeftOnlyStepsPhi_terminal_decompose_kdone_agree :
+  forall left right phi_state phi_left heap_final v_final,
+    state_heap left = state_heap right ->
+    PairParLeftOnlyStepsPhi
+      (PPS_Run left right KDone)
+      phi_state
+      phi_left
+      (PPS_State (StDone heap_final v_final)) ->
+    exists v_right heap_left v_left,
+      right = StDone (state_heap left) v_right /\
+      StepsPhi left phi_left (StDone heap_left v_left) /\
+      heap_final = heap_left /\
+      v_final = Pair (v_left, v_right).
+Proof.
+  intros left right phi_state phi_left heap_final v_final HAgree HSteps.
+  dependent induction HSteps generalizing left right heap_final v_final HAgree.
+  - destruct
+      (IHHSteps left' (with_state_heap (state_heap left') right)
+        heap_final v_final)
+      as (v_right & heap_left & v_left &
+          HRightDoneEq & HLeftSteps & HHeapFinal & HValFinal).
+    + rewrite state_heap_with_state_heap. reflexivity.
+    + reflexivity.
+    + reflexivity.
+    + destruct right as [heap_right env_right rho_right e_right k_right
+                       | heap_right v_right0 k_right
+                       | heap_right v_right0].
+      * simpl in HRightDoneEq. inversion HRightDoneEq.
+      * simpl in HRightDoneEq. inversion HRightDoneEq.
+      * simpl in HRightDoneEq. inversion HRightDoneEq; subst.
+        exists v_right, heap_left, v_left.
+        split.
+        -- simpl in HAgree. subst heap_right. reflexivity.
+        -- split.
+           ++ eapply StepsPhi_Step; eauto.
+           ++ split; reflexivity.
+  - destruct
+      (PairParLeftOnlyStepsPhi_state_as_stepsphi
+        (StReturn heap (Pair (v1, v2)) KDone)
+        phi_state phi_left
+        (PPS_State (StDone heap_final v_final)) HSteps)
+      as (HLeftNil & state_final & HStateFinal & HStateSteps).
+    inversion HStateFinal; subst.
+    destruct
+      (StepsPhi_terminal_deterministic
+        (StReturn heap (Pair (v1, v2)) KDone)
+        phi_state heap_final v_final
+        (Phi_Seq (label_phi Silent) Phi_Nil)
+        heap (Pair (v1, v2))
+        HStateSteps
+        (StepsPhi_return_kdone
+          heap (Pair (v1, v2))))
+      as (_ & HHeapEq & HValEq).
+    exists v2, heap, v1.
+    split.
+    + reflexivity.
+    + split.
+      * constructor.
+ 	      * split; assumption.
+Qed.
+
+Lemma PairParRightThenLeftStepsPhi_terminal_decompose_kdone :
+  forall left right phi_state phi_left phi_right heap_final v_final,
+    state_heap left = state_heap right ->
+    PairParRightThenLeftStepsPhi
+      (PPS_Run left right KDone)
+      phi_state
+      phi_left
+      phi_right
+      (PPS_State (StDone heap_final v_final)) ->
+    exists heap_right v_right heap_left v_left,
+      StepsPhi right phi_right (StDone heap_right v_right) /\
+      StepsPhi (with_state_heap heap_right left) phi_left
+        (StDone heap_left v_left) /\
+      heap_final = heap_left /\
+      v_final = Pair (v_left, v_right).
+Proof.
+  intros left right phi_state phi_left phi_right heap_final v_final
+    HAgree HSteps.
+  dependent induction HSteps generalizing left right heap_final v_final HAgree.
+  - destruct
+      (PairParLeftOnlyStepsPhi_terminal_decompose_kdone_agree
+        left right phi_state phi_left heap_final v_final HAgree H)
+      as (v_right & heap_left & v_left &
+          HRightDone & HLeftSteps & HHeapFinal & HValFinal).
+    exists (state_heap left), v_right, heap_left, v_left.
+    split.
+    + rewrite HRightDone. constructor.
+    + split.
+      * rewrite with_state_heap_state_heap. exact HLeftSteps.
+      * split; assumption.
+  - destruct
+      (IHHSteps
+        (with_state_heap (state_heap right') left)
+        right'
+        heap_final
+        v_final)
+      as (heap_right & v_right & heap_left & v_left &
+          HRightSteps & HLeftSteps & HHeapFinal & HValFinal).
+    + rewrite state_heap_with_state_heap. reflexivity.
+    + reflexivity.
+    + reflexivity.
+    + exists heap_right, v_right, heap_left, v_left.
+      split.
+      * eapply StepsPhi_Step; eauto.
+      * split.
+        -- rewrite with_state_heap_overwrite in HLeftSteps.
+           exact HLeftSteps.
+        -- split; assumption.
+Qed.
+
+Lemma Phi_Theta_Soundness_seq_inv_l :
+  forall phi1 phi2 theta,
+    Phi_Seq phi1 phi2 ⋞ theta ->
+    phi1 ⋞ theta.
+Proof.
+  intros phi1 phi2 theta HSound.
+  inversion HSound; subst; assumption.
+Qed.
+
+Lemma Phi_Theta_Soundness_seq_inv_r :
+  forall phi1 phi2 theta,
+    Phi_Seq phi1 phi2 ⋞ theta ->
+    phi2 ⋞ theta.
+Proof.
+  intros phi1 phi2 theta HSound.
+  inversion HSound; subst; assumption.
+Qed.
+
+Lemma PairParRightThenLeftStepsPhi_prepend_left :
+  forall left right k label left' phi_state phi_left phi_right final_state
+    theta_left theta_right,
+    state_heap left = state_heap right ->
+    Step left label left' ->
+    label_phi label ⋞ theta_left ->
+    phi_right ⋞ theta_right ->
+    PairParCheckPass theta_left theta_right ->
+    PairParRightThenLeftStepsPhi
+      (PPS_Run left' (with_state_heap (state_heap left') right) k)
+      phi_state phi_left phi_right final_state ->
+    PairParRightThenLeftStepsPhi
+      (PPS_Run left right k)
+      phi_state
+      (Phi_Seq (label_phi label) phi_left)
+      phi_right
+      final_state.
+Proof.
+  intros left right k label left' phi_state phi_left phi_right final_state
+    theta_left theta_right HHeapAgree HStepLeft HSoundLeft HSoundRight HPass HRTL.
+  remember
+    (PPS_Run left' (with_state_heap (state_heap left') right) k)
+    as rest_start eqn:HRestStart.
+  revert left right k label left' HHeapAgree HStepLeft HSoundLeft HRestStart.
+  induction HRTL;
+    intros left0 right0 k0 label0 left0' HHeapAgree HStepLeft HSoundLeft HRestStart;
+    inversion HRestStart; subst.
+  - apply PPRTL_LeftOnly.
+    eapply PPLO_Left.
+    + exact HStepLeft.
+    + assumption.
+  - pose proof
+      (Phi_Theta_Soundness_seq_inv_l
+        (label_phi label) phi_right theta_right HSoundRight)
+      as HSoundRightHead.
+    pose proof
+      (Phi_Theta_Soundness_seq_inv_r
+        (label_phi label) phi_right theta_right HSoundRight)
+      as HSoundRightTail.
+    destruct HPass as [HDisjointTheta HNoConflictTheta].
+    assert (HStable :
+      LabelAllocReflectionStable label label0).
+    {
+      eapply LabelAllocReflectionStable_from_theta; eauto.
+    }
+    assert (HDisjointLR :
+      Disjoint_Traces (label_trace label0) (label_trace label)).
+    {
+      rewrite <- (phi_as_list_label_phi label0).
+      rewrite <- (phi_as_list_label_phi label).
+      eapply PairParCheckPass_sound_disjoint_traces; eauto.
+      split; assumption.
+    }
+    assert (HDisjointRL :
+      Disjoint_Traces (label_trace label) (label_trace label0)).
+    {
+      rewrite <- (phi_as_list_label_phi label).
+      rewrite <- (phi_as_list_label_phi label0).
+      eapply PairParCheckPass_sound_disjoint_traces_sym; eauto.
+      split; assumption.
+    }
+    destruct
+      (PairParLeftRightActualStep_local_diamond
+        left0 right0 label0 label left0' right'
+        HHeapAgree HStepLeft H HStable HDisjointLR HDisjointRL)
+      as (right0' & HStepRight0 & HStepLeftAfterRight & HRightAfterRebase).
+    apply PPRTL_Right with (right' := right0').
+    + exact HStepRight0.
+    + eapply
+        (IHHRTL HSoundRightTail
+          (with_state_heap (state_heap right0') left0)
+          right0' k0 label0
+          (with_state_heap (state_heap right') left0')).
+      * rewrite state_heap_with_state_heap. reflexivity.
+      * exact HStepLeftAfterRight.
+      * exact HSoundLeft.
+      * rewrite state_heap_with_state_heap.
+        rewrite <- HRightAfterRebase.
+        reflexivity.
+Qed.
+
+Lemma PairParStepsPhi_normalize_right_then_left :
+  forall state phi_state phi_left phi_right final_state theta_left theta_right,
+    PairParRunHeapsAgree state ->
+    PairParStepsPhi state phi_state phi_left phi_right final_state ->
+    phi_left ⋞ theta_left ->
+    phi_right ⋞ theta_right ->
+    PairParCheckPass theta_left theta_right ->
+    PairParRightThenLeftStepsPhi
+      state phi_state phi_left phi_right final_state.
+Proof.
+  intros state phi_state phi_left phi_right final_state theta_left theta_right
+    HAgree HSteps.
+  induction HSteps;
+    intros HSoundLeft HSoundRight HPass.
+  - apply PPRTL_LeftOnly. constructor.
+  - assert (HWhole :
+      PairParStepsPhi
+        (PPS_State state)
+        (Phi_Seq (label_phi label) phi_state)
+        phi_left
+        phi_right
+        state'').
+    {
+      eapply PairParStepsPhi_State; eauto.
+    }
+    pose proof
+      (PairParStepsPhi_state_branches_nil
+        state (Phi_Seq (label_phi label) phi_state)
+        phi_left phi_right state'' HWhole)
+      as [HLeftNil HRightNil].
+    subst.
+    apply PPRTL_LeftOnly.
+    apply PPLO_State.
+    exact HWhole.
+  - pose proof
+      (Phi_Theta_Soundness_seq_inv_l
+        (label_phi label) phi_left theta_left HSoundLeft)
+      as HSoundLabel.
+    pose proof
+      (Phi_Theta_Soundness_seq_inv_r
+        (label_phi label) phi_left theta_left HSoundLeft)
+      as HSoundLeftTail.
+    eapply PairParRightThenLeftStepsPhi_prepend_left; eauto.
+    apply IHHSteps.
+    + simpl. rewrite state_heap_with_state_heap. reflexivity.
+    + exact HSoundLeftTail.
+    + exact HSoundRight.
+    + exact HPass.
+  - eapply PPRTL_Right.
+    + exact H.
+    + apply IHHSteps.
+      * simpl. rewrite state_heap_with_state_heap. reflexivity.
+      * exact HSoundLeft.
+      * eapply Phi_Theta_Soundness_seq_inv_r; eauto.
+      * exact HPass.
+  - pose proof
+      (PairParStepsPhi_state_branches_nil
+        (StReturn heap (Pair (v1, v2)) k)
+        phi_state phi_left phi_right state'' HSteps)
+      as [HLeftNil HRightNil].
+    subst.
+    apply PPRTL_LeftOnly.
+    eapply PPLO_Done.
+    apply PPLO_State.
+    exact HSteps.
+Qed.
+
+Theorem PairParCheckedArbitraryScheduleTerminalDeterminism :
+  forall heap env rho ef1 ea1 ef2 ea2
+    phi_state1 phi_left1 phi_right1
+    phi_state2 phi_left2 phi_right2
+    heap1 heap2 v1 v2 theta_left theta_right,
+    PairParCheckPass theta_left theta_right ->
+    phi_left1 ⋞ theta_left ->
+    phi_right1 ⋞ theta_right ->
+    phi_left2 ⋞ theta_left ->
+    phi_right2 ⋞ theta_right ->
+    PairParStepsPhi
+      (pairpar_checked_start heap env rho ef1 ea1 ef2 ea2 KDone)
+      phi_state1
+      phi_left1
+      phi_right1
+      (PPS_State (StDone heap1 v1)) ->
+    PairParStepsPhi
+      (pairpar_checked_start heap env rho ef1 ea1 ef2 ea2 KDone)
+      phi_state2
+      phi_left2
+      phi_right2
+      (PPS_State (StDone heap2 v2)) ->
+    heap1 = heap2 /\ v1 = v2.
+Proof.
+  intros heap env rho ef1 ea1 ef2 ea2
+    phi_state1 phi_left1 phi_right1
+    phi_state2 phi_left2 phi_right2
+    heap1 heap2 v1 v2 theta_left theta_right
+    HPass HSoundLeft1 HSoundRight1 HSoundLeft2 HSoundRight2
+    HSteps1 HSteps2.
+  assert (HAgreeStart :
+    PairParRunHeapsAgree
+      (pairpar_checked_start heap env rho ef1 ea1 ef2 ea2 KDone)).
+  {
+    unfold pairpar_checked_start, pairpar_checked_initial.
+    reflexivity.
+  }
+  pose proof
+    (PairParStepsPhi_normalize_right_then_left
+      (pairpar_checked_start heap env rho ef1 ea1 ef2 ea2 KDone)
+      phi_state1 phi_left1 phi_right1
+      (PPS_State (StDone heap1 v1))
+      theta_left theta_right
+      HAgreeStart HSteps1 HSoundLeft1 HSoundRight1 HPass)
+    as HRTL1.
+  pose proof
+    (PairParStepsPhi_normalize_right_then_left
+      (pairpar_checked_start heap env rho ef1 ea1 ef2 ea2 KDone)
+      phi_state2 phi_left2 phi_right2
+      (PPS_State (StDone heap2 v2))
+      theta_left theta_right
+      HAgreeStart HSteps2 HSoundLeft2 HSoundRight2 HPass)
+    as HRTL2.
+  unfold pairpar_checked_start, pairpar_checked_initial in HRTL1, HRTL2.
+  destruct
+    (PairParRightThenLeftStepsPhi_terminal_decompose_kdone
+      (initial_state heap env rho (Mu_App ef1 ea1))
+      (initial_state heap env rho (Mu_App ef2 ea2))
+      phi_state1 phi_left1 phi_right1 heap1 v1
+      eq_refl HRTL1)
+    as (heap_right1 & v_right1 & heap_left1 & v_left1 &
+        HRightSteps1 & HLeftSteps1 & HHeapFinal1 & HValFinal1).
+  destruct
+    (PairParRightThenLeftStepsPhi_terminal_decompose_kdone
+      (initial_state heap env rho (Mu_App ef1 ea1))
+      (initial_state heap env rho (Mu_App ef2 ea2))
+      phi_state2 phi_left2 phi_right2 heap2 v2
+      eq_refl HRTL2)
+    as (heap_right2 & v_right2 & heap_left2 & v_left2 &
+        HRightSteps2 & HLeftSteps2 & HHeapFinal2 & HValFinal2).
+  destruct
+    (StepsPhi_terminal_deterministic
+      (initial_state heap env rho (Mu_App ef2 ea2))
+      phi_right1 heap_right1 v_right1
+      phi_right2 heap_right2 v_right2
+      HRightSteps1 HRightSteps2)
+    as (_ & HRightHeapEq & HRightValEq).
+  subst heap_right2 v_right2.
+  destruct
+    (StepsPhi_terminal_deterministic
+      (with_state_heap heap_right1
+        (initial_state heap env rho (Mu_App ef1 ea1)))
+      phi_left1 heap_left1 v_left1
+      phi_left2 heap_left2 v_left2
+      HLeftSteps1 HLeftSteps2)
+    as (_ & HLeftHeapEq & HLeftValEq).
+  subst heap_left2 v_left2.
+  subst heap1 heap2 v1 v2.
+  split; reflexivity.
+Qed.
+
+Lemma PairParLeftRightStep_local_commute :
+  forall left right k label_left label_right left' right',
+    state_heap left = state_heap right ->
+    Step left label_left left' ->
+    Step right label_right right' ->
+    Disjoint_Traces (label_trace label_left) (label_trace label_right) ->
+    Disjoint_Traces (label_trace label_right) (label_trace label_left) ->
+    exists left_after right_after,
+      PairParStep
+        (PPS_Run left' (with_state_heap (state_heap left') right) k)
+        label_right
+        (PPS_Run (with_state_heap (state_heap right_after) left')
+           right_after k) /\
+      PairParStep
+        (PPS_Run (with_state_heap (state_heap right') left) right' k)
+        label_left
+        (PPS_Run left_after
+           (with_state_heap (state_heap left_after) right') k) /\
+      state_heap right_after ≡@{Heap} state_heap left_after.
+Proof.
+  intros left right k label_left label_right left' right'
+    HHeapAgree HStepLeft HStepRight HDisjointLR HDisjointRL.
+  pose
+    (right_after :=
+      with_state_heap
+        (label_result_heap label_right (state_heap left'))
+        right').
+  pose
+    (left_after :=
+      with_state_heap
+        (label_result_heap label_left (state_heap right'))
+        left').
+  exists left_after, right_after.
+  repeat split.
+  - subst right_after.
+    apply PPStep_Right.
+    eapply (Step_rebase_after_disjoint_step
+      right label_right right' left label_left left').
+    + symmetry. exact HHeapAgree.
+    + exact HStepRight.
+    + exact HStepLeft.
+    + exact HDisjointRL.
+  - subst left_after.
+    apply PPStep_Left.
+    eapply (Step_rebase_after_disjoint_step
+      left label_left left' right label_right right').
+    + exact HHeapAgree.
+    + exact HStepLeft.
+    + exact HStepRight.
+    + exact HDisjointLR.
+  - subst right_after left_after.
+    repeat rewrite state_heap_with_state_heap.
+    rewrite (Step_state_heap_label_result _ _ _ HStepLeft).
+    rewrite (Step_state_heap_label_result _ _ _ HStepRight).
+    rewrite <- HHeapAgree.
+    apply label_result_heap_commute_disjoint.
+    exact HDisjointLR.
+Qed.
+
+Theorem PairParCheckedSameProjectionScheduleHeapDeterminism :
+  forall heap env rho ef1 ea1 ef2 ea2
+    phi_state1 phi_state2 phi_left phi_right
+    heap1 heap2 v1 v2 theta_left theta_right,
+    PairParCheckPass theta_left theta_right ->
+    phi_left ⋞ theta_left ->
+    phi_right ⋞ theta_right ->
+    PairParStepsPhi
+      (pairpar_checked_start heap env rho ef1 ea1 ef2 ea2 KDone)
+      phi_state1
+      phi_left
+      phi_right
+      (PPS_State (StDone heap1 v1)) ->
+    PairParStepsPhi
+      (pairpar_checked_start heap env rho ef1 ea1 ef2 ea2 KDone)
+      phi_state2
+      phi_left
+      phi_right
+      (PPS_State (StDone heap2 v2)) ->
+    heap1 ≡@{Heap} heap2.
+Proof.
+  intros heap env rho ef1 ea1 ef2 ea2
+    phi_state1 phi_state2 phi_left phi_right
+    heap1 heap2 v1 v2 theta_left theta_right
+    HPass HSoundLeft HSoundRight HSteps1 HSteps2.
+  destruct
+    (PairParStepsPhi_branch_det_traces
+      (pairpar_checked_start heap env rho ef1 ea1 ef2 ea2 KDone)
+      phi_state1 phi_left phi_right
+      (PPS_State (StDone heap1 v1)) HSteps1)
+    as (HDetLeft & HDetRight).
+  pose proof
+    (PairParStepsPhi_top_terminal_state_trace_nil
+      heap env rho ef1 ea1 ef2 ea2
+      phi_state1 phi_left phi_right heap1 v1 HSteps1)
+    as HStateNil1.
+  pose proof
+    (PairParStepsPhi_top_terminal_state_trace_nil
+      heap env rho ef1 ea1 ef2 ea2
+      phi_state2 phi_left phi_right heap2 v2 HSteps2)
+    as HStateNil2.
+  unfold pairpar_checked_start, pairpar_checked_initial in HSteps1, HSteps2.
+  destruct
+    (PairParStepsPhi_run_split_replays_heap
+      (initial_state heap env rho (Mu_App ef1 ea1))
+      (initial_state heap env rho (Mu_App ef2 ea2))
+      KDone phi_state1 phi_left phi_right
+      (PPS_State (StDone heap1 v1))
+      eq_refl HSteps1)
+    as (heap_mid1 & HPar1 & HState1).
+  destruct
+    (PairParStepsPhi_run_split_replays_heap
+      (initial_state heap env rho (Mu_App ef1 ea1))
+      (initial_state heap env rho (Mu_App ef2 ea2))
+      KDone phi_state2 phi_left phi_right
+      (PPS_State (StDone heap2 v2))
+      eq_refl HSteps2)
+    as (heap_mid2 & HPar2 & HState2).
+  simpl in HState1, HState2.
+  pose proof
+    (unique_heap
+      heap heap_mid1 heap_mid2 phi_left phi_right theta_left theta_right
+      HSoundLeft HSoundRight HPass HDetLeft HDetRight HPar2 HPar1)
+    as HMidEq.
+  pose proof
+    (Phi_Heap_Steps_empty_as_list_preserves_heap
+      phi_state1 heap_mid1 heap1 HStateNil1 HState1)
+    as HFinal1.
+  pose proof
+    (Phi_Heap_Steps_empty_as_list_preserves_heap
+      phi_state2 heap_mid2 heap2 HStateNil2 HState2)
+    as HFinal2.
+  transitivity heap_mid1.
+  - symmetry. exact HFinal1.
+  - transitivity heap_mid2; assumption.
+Qed.
+
+Theorem PairParCheckedSameProjectionScheduleTerminalHeapAndPairShape :
+  forall heap env rho ef1 ea1 ef2 ea2
+    phi_state1 phi_state2 phi_left phi_right
+    heap1 heap2 v1 v2 theta_left theta_right,
+    PairParCheckPass theta_left theta_right ->
+    phi_left ⋞ theta_left ->
+    phi_right ⋞ theta_right ->
+    PairParStepsPhi
+      (pairpar_checked_start heap env rho ef1 ea1 ef2 ea2 KDone)
+      phi_state1
+      phi_left
+      phi_right
+      (PPS_State (StDone heap1 v1)) ->
+    PairParStepsPhi
+      (pairpar_checked_start heap env rho ef1 ea1 ef2 ea2 KDone)
+      phi_state2
+      phi_left
+      phi_right
+      (PPS_State (StDone heap2 v2)) ->
+    heap1 ≡@{Heap} heap2 /\
+    (exists v1_left v1_right,
+      v1 = Pair (v1_left, v1_right)) /\
+    (exists v2_left v2_right,
+      v2 = Pair (v2_left, v2_right)).
+Proof.
+  intros heap env rho ef1 ea1 ef2 ea2
+    phi_state1 phi_state2 phi_left phi_right
+    heap1 heap2 v1 v2 theta_left theta_right
+    HPass HSoundLeft HSoundRight HSteps1 HSteps2.
+  split.
+  - eapply PairParCheckedSameProjectionScheduleHeapDeterminism; eauto.
+  - split.
+    + unfold pairpar_checked_start, pairpar_checked_initial in HSteps1.
+      eapply PairParStepsPhi_run_kdone_terminal_pair_value; eauto.
+    + unfold pairpar_checked_start, pairpar_checked_initial in HSteps2.
+      eapply PairParStepsPhi_run_kdone_terminal_pair_value; eauto.
+Qed.
